src/Bedrock/P256/Jacobian.v
@@ -20,14 +20,14 @@ ProgramLogic WeakestPrecondition
 ProgramLogic.Coercions
 Word.Interface OfListWord Separation SeparationLogic
 letexists
-BasicC64Semantics
 ListIndexNotations
 SepAutoArray
 symmetry
 PeanoNat micromega.Lia
 Tactics
 UniquePose
-micromega.Lia Word.Properties.
+micromega.Lia Word.Properties
+bedrock2.BasicCSemantics.
 
 Require Import  Coq.Lists.List.
 
@@ -44,48 +44,29 @@ Import (notations) coqutil.Map.Memory.
 Import Coq.micromega.Lia.
 Import coqutil.Tactics.Tactics.
 
+Require Import bedrock2Examples.memcpy.
+
+(* Parameterize word size to ensure proofs are valid in 32 and 64 bit context.*)
+Section WithParameters.
+Context {width} {BW: Bitwidth.Bitwidth width}.
+#[local] Hint Extern 0 (word width) => exact (Naive.word width) : typeclass_instances.
+#[local] Notation word := (Naive.word width).
+
+Import Specs. (* Now word is accessible with short name. *)
+
+(* Now how do we get the more generic functions in. *)
+
+
+(* ZnWords with destructed word size equality after ZnWords_pre, to incorporate word size in hypothesis. *)
+#[local] Ltac ZnWords ::=
+  pose proof word_ok;  cbv [word] in *;
+  destruct Bitwidth.width_cases as [W|W]; symmetry in W; ZnWords_pre; try destruct W; better_lia.
+
+
 Definition p256_point_iszero := func! (p_P) ~> z {
   unpack! nz = p256_coord_nonzero(p_P.+$32.+$32);
   z = ~nz
 }.
-
-
-Lemma p256_point_iszero_ok : program_logic_goal_for_function! p256_point_iszero.
-Proof.
-  cbv [spec_of_fiat_p256_point_iszero].
-  repeat straightline.
-
-  rename H0 into Hm.
-  cbv [point.to_bytes] in *.
-  repeat seprewrite_in_by (@Array.sep_eq_of_list_word_at_app) Hm ltac:(rewrite ?app_length, ?length_coord; trivial; try lia).
-  simpl Z.of_nat in *.
-
-  straightline_call; [eexists; ecancel_assumption|]; repeat straightline.
-
-  subst z x0.
-  setoid_rewrite word.not_broadcast; rewrite Bool.negb_involutive; trivial.
-Qed.
-
-Definition p256_point_set_zero := func! (p_P) {
-  br_memset(p_P, $0, $(3*32))
-}.
-
-Lemma p256_point_set_zero_ok : program_logic_goal_for_function! p256_point_set_zero.
-Proof.
-  cbv [spec_of_p256_point_set_zero].
-  repeat straightline.
-
-  cbv [point.to_bytes] in *.
-
-  straightline_call; ssplit.
-  { ecancel_assumption. }
-  { ZnWords. }
-  repeat straightline.
-
-  cbv [fst snd proj1_sig Jacobian.of_affine Jacobian.of_affine_impl W.zero coord.to_bytes].
-  rewrite List.le_split_0_r. rewrite <- !repeat_app.
-  use_sep_assumption. Morphisms.f_equiv.
-Qed.
 
 Definition p256_coord_halve := func!(y, x) {
   stackalloc 32 as mmh;
@@ -94,103 +75,6 @@ Definition p256_coord_halve := func!(y, x) {
   u256_shr(y, x, $1);
   p256_coord_sub(y, y, mmh)
 }.
-
-Local Ltac length_tac :=
-  repeat rewrite
-    ?length_coord, ?length_point,
-    ?app_length, ?firstn_length, ?skipn_length, ?length_le_split, ?length_nil,
-    ?Nat.min_l
-    by (trivial; lia); trivial; lia.
-
-Lemma p256_coord_halve_ok :
-  let '_ := spec_of_p256_coord_sub_nonmont in
-  program_logic_goal_for_function! p256_coord_halve.
-Proof.
-  cbv [spec_of_p256_coord_halve].
-  straightline; repeat straightline_cleanup.
-
-  pose proof (conj H3 H4) as Hm; clear H4 H3; pattern m in Hm.
-  progress change (?P m) with (id P m) in Hm.
-  repeat straightline.
-  eapply sep_and_l_fwd in Hm; case Hm as [Hm Hm'].
-
-  letexists; split.
-  { cbn. repeat straightline. eexists; split; [|reflexivity].
-    cbv [coord.to_bytes] in Hm.
-    rewrite <-(firstn_skipn 8 (le_split _ _)), List.firstn_le_split, skipn_le_split, ?Z.shiftr_shiftr in Hm by lia.
-    seprewrite_in_by (@Array.sep_eq_of_list_word_at_app) Hm ltac:(rewrite ?length_le_split; trivial; lia).
-    seprewrite_in_by (symmetry! @Array.array1_iff_eq_of_list_word_at) Hm ltac:(rewrite ?length_le_split; lia).
-    seprewrite_in_by @Scalars.scalar_of_bytes Hm ltac:(rewrite ?length_le_split; lia).
-    rewrite le_combine_split in Hm.
-    repeat straightline. }
-
-  straightline_call; [eexists; ecancel_assumption|]; repeat straightline.
-
-  seprewrite_in_by Array.array1_iff_eq_of_list_word_at Hm0 ltac:(Lia.lia).
-
-  straightline_call; ssplit; [ ecancel_assumption | trivial | exact eq_refl | ].
-  repeat straightline.
-
-  eapply sep_and_r_fwd in H10; case H10 as [Hm3 Hm3'].
-
-  straightline_call; ssplit.
-  { eexists. cbv [coord.to_bytes] in *. ecancel_assumption. }
-  { cbv [coord.to_bytes] in *. ecancel_assumption. }
-  { trivial. }
-  { eapply F.to_Z_range, eq_refl. }
-  { etransitivity; try eapply F.to_Z_range; eapply eq_refl. }
-  { ZnWords.ZnWords. }
-
-  repeat straightline.
-  rewrite ?Z.pow_1_r in *.
-
-  set (Z.odd _) as b in *.
-
-  eapply WeakestPreconditionProperties.Proper_call; cycle -1;
-  [ eapply H2 | .. | intros ? ? ? ?]; ssplit.
-  { eexists.
-    use_sep_assumption; cancel.
-    cancel_seps_at_indices 0%nat 0%nat; [|cancel].
-
-    instantiate (1:=F.of_Z _ (F.to_Z (x*coord.R)%F / 2)).
-    rewrite F.to_Z_of_Z, Z.mod_small; trivial.
-    specialize (F.to_Z_range (x*coord.R) eq_refl); clear; PreOmega.Z.to_euclidean_division_equations; lia. }
-  { eexists. use_sep_assumption. cancel.
-    cancel_seps_at_indices 1%nat 0%nat. { exact eq_refl. }
-    cancel. }
-  { ecancel_assumption. }
-  { length_tac. }
-
-  repeat straightline.
-
-  (* stackdealloc *)
-  progress repeat seprewrite_in_by (symmetry! @Array.array1_iff_eq_of_list_word_at) H12 length_tac.
-  progress repeat match type of H12 with context [Array.array ptsto _ _ (le_split 32 ?x)] =>
-    unique pose proof (length_le_split 32 x) end.
-  progress repeat straightline.
-  progress repeat seprewrite_in_by (@Array.array1_iff_eq_of_list_word_at) H12 length_tac.
-
-  (* postcondition *)
-  use_sep_assumption.
-  cancel.
-  cancel_seps_at_indices 0%nat 0%nat; [|cancel].
-  f_equal.
-  f_equal.
-  subst x2 b.
-  cbv [coord.to_bytes F.div].
-  progress Morphisms.f_equiv; [].
-  progress Morphisms.f_equiv; [].
-  transitivity (x * coord.R * F.inv (1 + 1))%F; [|ring].
-  set (x*coord.R)%F as xR; set (F.inv (1 + 1)) as i2.
-
-  (* NOTE: back-and-forth rewrite between Z.modulo and Z.odd *)
-  rewrite word.unsigned_of_Z; cbv [word.wrap]; rewrite Zmod_mod, Zdiv.Zodd_mod, Z.mod_mod_divide by (apply Divide.Z.divide_pow_le with (n:=1); lia).
-  symmetry; rewrite <-(F.of_Z_to_Z xR) at 1; rewrite (Z.div_mod xR 2) at 1 by lia.
-  rewrite Div.Z.div_sub_mod_exact, Zdiv.Zmod_odd by lia.
-
-  assert (F.of_Z p256 2 * i2 = F.one)%F as Hi2 by (cbv [i2]; clear; Decidable.vm_decide).
-  case Z.odd; cbn [Z.eqb Pos.eqb Zeq_bool Z.compare Pos.compare Pos.compare_cont]; rewrite ?F.of_Z_add, ?F.of_Z_mul; fold (@F.zero p256); fold (@F.one p256); try ring [Hi2].
-Qed.
 
 Definition p256_point_add_nz_nz_neq := func! (p_out, p_P, p_Q) ~> ok {
   stackalloc 32 as z1z1;
@@ -233,77 +117,6 @@ Definition p256_point_add_nz_nz_neq := func! (p_out, p_P, p_Q) ~> ok {
   p256_coord_sub(p_out.+$32, h, s2)
 }.
 
-Lemma p256_point_add_nz_nz_neq_ok : program_logic_goal_for_function! p256_point_add_nz_nz_neq.
-Proof.
-  cbv [spec_of_p256_point_add_nz_nz_neq].
-  straightline; repeat straightline_cleanup.
-  destruct P as (((x1 & y1) & z1) & p1),  Q as (((x2 & y2) & z2) & p2);
-    cbv [proj1_sig proj2_sig fst snd point.to_bytes] in * |-.
-  repeat seprewrite_in_by Array.sep_eq_of_list_word_at_app H25
-     ltac:(rewrite ?app_length, ?length_coord; trivial; try Lia.lia).
-
-  repeat straightline.
-  repeat seprewrite_in_by Array.array1_iff_eq_of_list_word_at H25 ltac:(Lia.lia).
-
-  rewrite <-(firstn_skipn 32 out) in H25.
-  rewrite <-(firstn_skipn 32 (skipn _ out)) in H25.
-  rewrite ?skipn_skipn in H25.
-rewrite ?app_length, ?length_coord in *.
-  repeat seprewrite_in_by Array.sep_eq_of_list_word_at_app H25 (* WHY does first rewrite take 0.1s? *)
-    ltac:(repeat rewrite ?app_length, ?firstn_length, ?skipn_length, ?Nat.min_l; try Lia.lia; trivial).
-
-  progress change (Z.of_nat 32) with 32 in *.
-
-  repeat (straightline_call; ssplit;
-    [ solve [repeat match goal with
-      | |- True => exact I
-      | |- exists _, _ => letexists
-      | |- _ => progress rewrite ?length_coord, ?firstn_length, ?skipn_length; ZnWords
-      | _ => ecancel_assumption
-      end] ..
-    | repeat straightline ]).
-
-  (* stackdealloc *)
-  progress repeat seprewrite_in_by (symmetry! @Array.array1_iff_eq_of_list_word_at) H93 ltac:(rewrite ?length_coord; Lia.lia).
-  progress repeat match type of H93 with context [Array.array ptsto _ _ (coord.to_bytes ?x)] =>
-    unique pose proof (length_coord x) end.
-  repeat straightline.
-  progress repeat seprewrite_in_by (@Array.array1_iff_eq_of_list_word_at) H93 ltac:(rewrite ?length_coord; Lia.lia).
-
-  (* postcondition *)
-  eexists; ssplit.
-  {
-    cbv [proj1_sig proj2_sig fst snd point.to_bytes].
-    repeat seprewrite_in_by Array.list_word_at_app_of_adjacent_eq H93 ltac:(rewrite ?length_coord; listZnWords).
-    (* other direction: repeat seprewrite_by Array.sep_eq_of_list_word_at_app ltac:(rewrite ?length_coord, ?app_length; trivial; try Lia.lia). *)
-    ecancel_assumption. }
-  { rewrite ?app_length, ?length_point, ?length_coord; trivial. }
-
-  case (Properties.word.eqb_spec x3 (word.of_Z 0)); subst x3; rewrite word.lor_0_iff; [right|left]; split; trivial.
-  { case H121 as [Hx Hy].
-    subst x x0.
-    rewrite !word.broadcast_0_iff in *.
-    rewrite !Bool.negb_false_iff, !F.eqb_eq in *.
-    cbv [fst snd Jacobian.eq Jacobian.iszero proj1_sig] in *.
-    case Decidable.dec; intros; try contradiction; split; trivial.
-    rewrite Hierarchy.commutative in Hx.
-    rewrite <-!F.pow_succ_r in Hx, Hy; simpl N.succ in Hx, Hy.
-    rewrite F.pow_0_iff, Ring.sub_zero_iff in Hx, Hy by (lia||exact _).
-    rewrite ?F.pow_3_r, ?F.pow_2_r in Hx.
-    rewrite ?F.pow_3_r, ?F.pow_2_r in Hy.
-    split; Field.fsatz. }
-  { unshelve eexists ?[pfPneqQ].
-    { intros HX; cbv [Jacobian.eq Jacobian.iszero proj1_sig fst snd] in H122, H123, HX.
-      destruct Decidable.dec in HX; try contradiction; case HX as (Hz&Hx&Hy).
-      apply H121. subst x x0.
-      rewrite !word.broadcast_0_iff in *.
-      rewrite !Bool.negb_false_iff, !F.eqb_eq.
-      rewrite ?F.pow_3_r, ?F.pow_2_r, ?Hx, ?Hy, ?(proj2 (Ring.sub_zero_iff _ _)); ssplit; Field.fsatz. }
-    cbv [Jacobian.add_inequal_nz_nz point.to_bytes]; cbn [fst snd proj1_sig].
-    rewrite ?F.pow_3_r, ?F.pow_2_r.
-    trivial. }
-Qed.
-
 Definition p256_point_add_vartime_if_doubling := func!(p_out, p_P, p_Q) {
   unpack! zeroP = p256_point_iszero(p_P);
   unpack! zeroQ = p256_point_iszero(p_Q);
@@ -319,11 +132,269 @@ Definition p256_point_add_vartime_if_doubling := func!(p_out, p_P, p_Q) {
   br_memcpy(p_out, p_sel, $(3*32))
 }.
 
-#[local] Ltac ensure_map m := lazymatch type of m with | @Interface.map.rep _ _ _ => true | _ => false end.
-#[local] Ltac newest_memory_hyp := match goal with | H: ?G ?m |- _ =>
-match (ensure_map m) with true => H | false => fail end end.
+Definition p256_point_double := func!(out, in1) {
+  stackalloc 32 as D;
+  stackalloc 32 as A;
+  stackalloc 32 as tmp;
+  p256_coord_add(D, in1.+$32, in1.+$32);
+  p256_coord_sqr(tmp, in1.+$32.+$32);
+  p256_coord_sqr(D, D);
+  p256_coord_mul(out.+$32.+$32, in1.+$32.+$32, in1.+$32);
+  p256_coord_add(out.+$32.+$32, out.+$32.+$32, out.+$32.+$32);
+  p256_coord_add(A, in1, tmp);
+  p256_coord_sub(tmp, in1, tmp);
+  { stackalloc 32 as t2; p256_coord_add(t2, tmp, tmp); p256_coord_add(tmp, t2, tmp) };
+  p256_coord_sqr(out.+$32, D);
+  p256_coord_mul(A, A, tmp);
+  p256_coord_mul(D, D, in1);
+  p256_coord_sqr(out, A);
+  p256_coord_add(tmp, D, D);
+  p256_coord_sub(out, out, tmp);
+  p256_coord_sub(D, D, out);
+  p256_coord_mul(D, D, A);
+  p256_coord_halve(out.+$32, out.+$32);
+  p256_coord_sub(out.+$32, D, out.+$32)
+}.
 
-Import memcpy.
+Definition p256_point_set_zero := func! (p_P) {
+  br_memset(p_P, $0, $(3*32))
+}.
+
+#[local] Ltac ensure_map m := lazymatch type of m with | @Interface.map.rep _ _ _ => true | _ => false end.
+#[local] Ltac contains_sep P := match P with context [sep] => true | _ => false end.
+#[local] Ltac oldest_memory_hyp := match reverse goal with | H: ?G ?m |- _ =>
+  match (ensure_map m) with
+    | true => match (contains_sep G) with
+        | true => H
+        | false => fail
+      end
+    | false => fail end end.
+#[local] Ltac newest_memory_hyp := match goal with | H: ?G ?m |- _ =>
+  match (ensure_map m) with true => H | false => fail end end.
+#[local] Ltac clear_old_memory_hyps := repeat (
+  let Hold := oldest_memory_hyp in
+  let Hnew := newest_memory_hyp in
+  lazymatch Hold with Hnew => fail | _ => clear Hold end
+).
+
+Lemma p256_point_iszero_ok : program_logic_goal_for_function! p256_point_iszero.
+Proof.
+  cbv [spec_of_fiat_p256_point_iszero].
+
+  repeat straightline.
+
+  rename H0 into Hm.
+  cbv [point.to_bytes] in *.
+  repeat seprewrite_in_by (@Array.sep_eq_of_list_word_at_app) Hm ltac:(rewrite ?app_length, ?length_coord; trivial; try ZnWords).
+  simpl Z.of_nat in *.
+
+  straightline_call; [eexists; ecancel_assumption|]; repeat straightline.
+
+  subst z x0.
+  setoid_rewrite word.not_broadcast; rewrite Bool.negb_involutive; trivial.
+Qed.
+
+Lemma p256_point_set_zero_ok : program_logic_goal_for_function! p256_point_set_zero.
+Proof.
+  cbv [spec_of_p256_point_set_zero].
+  repeat straightline.
+
+  cbv [point.to_bytes] in *.
+
+  straightline_call; ssplit.
+  { ecancel_assumption. }
+  { ZnWords. }
+  repeat straightline.
+
+  cbv [fst snd proj1_sig Jacobian.of_affine Jacobian.of_affine_impl W.zero coord.to_bytes].
+  rewrite List.le_split_0_r. rewrite <- !repeat_app.
+  use_sep_assumption. do 2 Morphisms.f_equiv. do 2 f_equal. ZnWords.
+Qed.
+
+Local Ltac length_tac :=
+  repeat rewrite
+    ?length_coord, ?length_point,
+    ?app_length, ?firstn_length, ?skipn_length, ?length_le_split, ?length_nil,
+    ?Nat.min_l
+    by (trivial; lia); trivial; (lia || ZnWords).
+
+Lemma p256_coord_halve_ok :
+  let '_ := spec_of_p256_coord_sub_nonmont in
+  program_logic_goal_for_function! p256_coord_halve.
+Proof.
+  cbv [spec_of_p256_coord_halve].
+  straightline; repeat straightline_cleanup.
+
+  pose proof (conj H3 H4) as Hm; clear H4 H3; pattern m in Hm.
+  progress change (?P m) with (id P m) in Hm.
+  repeat straightline.
+
+  split; [destruct Bitwidth.width_cases as [W | W]; rewrite W; cbn; lia|].
+
+  repeat straightline.
+
+  eapply sep_and_l_fwd in Hm; case Hm as [Hm Hm'].
+
+  letexists; split.
+  { cbn. repeat straightline. eexists; split; [|reflexivity].
+    cbv [coord.to_bytes] in Hm.
+    rewrite <-(firstn_skipn (Z.to_nat (Memory.bytes_per_word width)) (le_split _ _)), List.firstn_le_split, skipn_le_split, ?Z.shiftr_shiftr in Hm by (unfold Memory.bytes_per_word; ZnWords).
+    seprewrite_in_by (@Array.sep_eq_of_list_word_at_app) Hm ltac:(rewrite ?length_le_split; trivial; ZnWords).
+    seprewrite_in_by (symmetry! @Array.array1_iff_eq_of_list_word_at) Hm ltac:(rewrite ?length_le_split; ZnWords).
+    seprewrite_in @Scalars.scalar_of_bytes Hm.
+    { rewrite length_le_split. unfold Memory.bytes_per_word. ZnWords. }
+    rewrite le_combine_split in Hm.
+    repeat straightline. }
+
+  straightline_call; [eexists; ecancel_assumption|]; repeat straightline.
+
+  seprewrite_in_by @Array.array1_iff_eq_of_list_word_at Hm0 ltac:(ZnWords).
+
+  straightline_call; ssplit; [ ecancel_assumption | trivial | exact eq_refl | ].
+  repeat straightline.
+
+  eapply sep_and_r_fwd in H10; case H10 as [Hm3 Hm3'].
+
+  straightline_call; ssplit.
+  { eexists. cbv [coord.to_bytes] in *. ecancel_assumption. }
+  { cbv [coord.to_bytes] in *. ecancel_assumption. }
+  { trivial. }
+  { eapply F.to_Z_range, eq_refl. }
+  { etransitivity; try eapply F.to_Z_range; eapply eq_refl. }
+  { ZnWords.ZnWords. }
+
+  repeat straightline.
+  rewrite ?Z.pow_1_r in *.
+
+  set (Z.odd _) as b in *.
+
+  eapply WeakestPreconditionProperties.Proper_call; cycle -1;
+  [ eapply H2 | .. | intros ? ? ? ?]; ssplit.
+  { eexists.
+    use_sep_assumption; cancel.
+    cancel_seps_at_indices 0%nat 0%nat; [|cancel].
+    rewrite word.unsigned_of_Z_1.
+    instantiate (1:=F.of_Z _ (F.to_Z (x*coord.R)%F / 2)).
+    rewrite F.to_Z_of_Z.
+    rewrite Z.mod_small. { trivial. }
+    specialize (F.to_Z_range (x*coord.R) eq_refl); clear; PreOmega.Z.to_euclidean_division_equations; lia. }
+  { eexists. use_sep_assumption. cancel.
+    cancel_seps_at_indices 1%nat 0%nat. { exact eq_refl. }
+    cancel. }
+  { ecancel_assumption. }
+  { length_tac. }
+
+  repeat straightline.
+
+  (* stackdealloc *)
+  progress repeat seprewrite_in_by (symmetry! @Array.array1_iff_eq_of_list_word_at) H12 length_tac.
+  progress repeat match type of H12 with context [Array.array ptsto _ _ (le_split 32 ?x)] =>
+    unique pose proof (length_le_split 32 x) end.
+  progress repeat straightline.
+  progress repeat seprewrite_in_by (@Array.array1_iff_eq_of_list_word_at) H12 length_tac.
+
+  (* postcondition *)
+  use_sep_assumption.
+  cancel.
+  cancel_seps_at_indices 0%nat 0%nat; [|cancel].
+  apply (f_equal sepclause_of_map).
+  apply (f_equal (map.of_list_word_at p_out)).
+  subst x2 b.
+  cbv [coord.to_bytes F.div].
+  progress Morphisms.f_equiv; [].
+  progress Morphisms.f_equiv; [].
+  transitivity (x * coord.R * F.inv (1 + 1))%F; [|ring].
+  set (x*coord.R)%F as xR; set (F.inv (1 + 1)) as i2.
+
+  assert (Z.of_nat (Nat.min (Z.to_nat (Memory.bytes_per_word width)) 32) * 8 = width) as -> by (destruct Bitwidth.width_cases as [J|J]; rewrite J; cbv; reflexivity).
+  rewrite word.unsigned_of_Z; cbv [word.wrap].
+  rewrite Zmod_mod, Zdiv.Zodd_mod, Z.mod_mod_divide by (apply Divide.Z.divide_pow_le with (n:=1); ZnWords).
+  symmetry; rewrite <-(F.of_Z_to_Z xR) at 1; rewrite (Z.div_mod xR 2) at 1 by lia.
+  rewrite Div.Z.div_sub_mod_exact, Zdiv.Zmod_odd by lia.
+
+  assert (F.of_Z p256 2 * i2 = F.one)%F as Hi2 by (cbv [i2]; clear; Decidable.vm_decide).
+  case Z.odd; cbn [Z.eqb Pos.eqb Zeq_bool Z.compare Pos.compare Pos.compare_cont]; rewrite ?F.of_Z_add, ?F.of_Z_mul; fold (@F.zero p256); fold (@F.one p256); try ring [Hi2].
+Qed.
+
+Lemma p256_point_add_nz_nz_neq_ok : program_logic_goal_for_function! p256_point_add_nz_nz_neq.
+Proof.
+  cbv [spec_of_p256_point_add_nz_nz_neq].
+  straightline; repeat straightline_cleanup.
+  destruct P as (((x1 & y1) & z1) & p1),  Q as (((x2 & y2) & z2) & p2);
+    cbv [proj1_sig proj2_sig fst snd point.to_bytes] in * |-.
+  repeat seprewrite_in_by Array.sep_eq_of_list_word_at_app H25
+     ltac:(rewrite ?app_length, ?length_coord; trivial; try ZnWords).
+
+  repeat straightline.
+
+  repeat (split;
+  (* TODO Generalize if used more often. This is alignment of 32 bytes with width. *)
+  [ unfold Memory.bytes_per_word; destruct Bitwidth.width_cases as [W | W]; rewrite W; cbv; lia |
+  repeat straightline]).
+
+  repeat seprewrite_in_by @Array.array1_iff_eq_of_list_word_at H25 ltac:(ZnWords).
+
+  rewrite <-(firstn_skipn 32 out) in H25.
+  rewrite <-(firstn_skipn 32 (skipn _ out)) in H25.
+  rewrite ?skipn_skipn in H25.
+  rewrite ?app_length, ?length_coord in *.
+  clear_old_memory_hyps.
+  repeat seprewrite_in_by @Array.sep_eq_of_list_word_at_app H25 (* WHY does first rewrite take 0.1s? *)
+    ltac:(repeat rewrite ?app_length, ?firstn_length, ?skipn_length, ?length_coord, ?Nat.min_l; try ZnWords; trivial).
+
+  progress change (Z.of_nat 32) with 32 in *.
+
+  repeat (clear_old_memory_hyps; straightline_call; ssplit;
+    [ solve [repeat match goal with
+      | |- True => exact I
+      | |- exists _, _ => letexists
+      | |- _ => progress rewrite ?length_coord, ?firstn_length, ?skipn_length; ZnWords
+      | _ => ecancel_assumption
+      end] ..
+    | repeat straightline ]).
+
+  (* stackdealloc *)
+  progress repeat seprewrite_in_by (symmetry! @Array.array1_iff_eq_of_list_word_at) ltac:(newest_memory_hyp) ltac:(rewrite ?length_coord; ZnWords).
+  let H := newest_memory_hyp in progress repeat match type of H with context [Array.array ptsto _ _ (coord.to_bytes ?x)] =>
+    unique pose proof (length_coord x) end.
+  repeat straightline.
+  clear_old_memory_hyps.
+  progress repeat seprewrite_in_by (@Array.array1_iff_eq_of_list_word_at) ltac:(newest_memory_hyp) ltac:(rewrite ?length_coord; ZnWords).
+
+  (* postcondition *)
+  eexists; ssplit.
+  {
+    cbv [proj1_sig proj2_sig fst snd point.to_bytes].
+    repeat seprewrite_in_by @Array.list_word_at_app_of_adjacent_eq ltac:(newest_memory_hyp) ltac:(rewrite ?length_coord; listZnWords).
+    ecancel_assumption. }
+  { rewrite ?app_length, ?length_point, ?length_coord; trivial. }
+
+  case (Properties.word.eqb_spec x3 (word.of_Z 0)); subst x3; rewrite word.lor_0_iff; [right|left]; split; trivial.
+  { match goal with H: _ /\ _ |- _=> case H as [Hx Hy] end.
+    subst x x0.
+    rewrite !word.broadcast_0_iff in *.
+    rewrite !Bool.negb_false_iff, !F.eqb_eq in *.
+    cbv [fst snd Jacobian.eq Jacobian.iszero proj1_sig] in *.
+    case Decidable.dec; intros; try contradiction; split; trivial.
+    rewrite Hierarchy.commutative in Hx.
+    rewrite <-!F.pow_succ_r in Hx, Hy; simpl N.succ in Hx, Hy.
+    rewrite F.pow_0_iff, Ring.sub_zero_iff in Hx, Hy by (lia||exact _).
+    rewrite ?F.pow_3_r, ?F.pow_2_r in Hx.
+    rewrite ?F.pow_3_r, ?F.pow_2_r in Hy.
+    split; Field.fsatz. }
+  { unshelve eexists ?[pfPneqQ].
+    { intros HX; cbv [Jacobian.eq Jacobian.iszero proj1_sig fst snd] in *.
+      destruct Decidable.dec in HX; try contradiction; case HX as (Hz&Hx&Hy).
+      match goal with H: ~(_ /\ _) |- _=> apply H end.
+      subst x x0.
+      rewrite !word.broadcast_0_iff.
+      rewrite !Bool.negb_false_iff, !F.eqb_eq.
+      rewrite ?F.pow_3_r, ?F.pow_2_r, ?Hx, ?Hy, ?(proj2 (Ring.sub_zero_iff _ _)); ssplit; Field.fsatz. }
+    cbv [Jacobian.add_inequal_nz_nz point.to_bytes]; cbn [fst snd proj1_sig].
+    rewrite ?F.pow_3_r, ?F.pow_2_r.
+    trivial. }
+Qed.
+
 Lemma p256_point_add_vartime_if_doubling_ok :
   let spec := spec_of_p256_point_add_vartime_if_doubling in
   program_logic_goal_for_function! p256_point_add_vartime_if_doubling.
@@ -336,25 +407,33 @@ Proof.
   straightline_call; repeat straightline. (*iszero*)
   { eexists. ecancel_assumption. }
   (* stackalloc *)
-  seprewrite_in_by (@Array.array1_iff_eq_of_list_word_at) ltac:(newest_memory_hyp) ltac:(lia).
+  split.
+  (* TODO Generalize if used more often. This is alignment of 32 bytes with width. *)
+  { unfold Memory.bytes_per_word. destruct Bitwidth.width_cases as [W | W]; rewrite W; cbv; lia. }
+  repeat straightline.
+  seprewrite_in_by (@Array.array1_iff_eq_of_list_word_at) ltac:(newest_memory_hyp) ltac:(ZnWords).
   straightline_call; ssplit. (*add*)
   { ecancel_assumption. }
   { lia. }
   repeat straightline.
   straightline_call; repeat straightline (* br_declassify *).
   (* stackalloc *)
-  seprewrite_in_by (@Array.array1_iff_eq_of_list_word_at) ltac:(newest_memory_hyp) ltac:(lia).
+  split.
+  (* TODO Generalize if used more often. This is alignment of 32 bytes with width. *)
+  { unfold Memory.bytes_per_word. destruct Bitwidth.width_cases as [W | W]; rewrite W; cbv; lia. }
+  repeat straightline.
+  seprewrite_in_by (@Array.array1_iff_eq_of_list_word_at) ltac:(newest_memory_hyp) ltac:(ZnWords).
   straightline_call; ssplit. (* memset *)
   { ecancel_assumption. }
   { ZnWords. }
   repeat straightline.
   straightline_call; repeat straightline; ssplit (* memcxor *).
   { ecancel_assumption. }
-  { rewrite ?repeat_length; trivial. }
+  { rewrite ?repeat_length; ZnWords. }
   { ZnWords. }
   straightline_call; repeat straightline; ssplit (* memcxor *).
   { ecancel_assumption. }
-  { rewrite ?repeat_length; trivial. }
+  { rewrite ?repeat_length; ZnWords. }
   { ZnWords. }
   straightline_call; repeat straightline; ssplit (* memcxor *).
   { ecancel_assumption. }
@@ -366,7 +445,7 @@ Proof.
     { ecancel_assumption. }
     { ZnWords. }
     { trivial. }
-    { clear; ZnWords. }
+    { ZnWords. }
     repeat straightline.
     (* stackdealloc *)
     progress repeat seprewrite_in_by (symmetry! @Array.array1_iff_eq_of_list_word_at) ltac:(newest_memory_hyp)
@@ -374,20 +453,20 @@ Proof.
     assert (Datatypes.length x6 = 96%nat) by ZnWords.ZnWords.
     repeat straightline.
     progress repeat seprewrite_in_by (@Array.array1_iff_eq_of_list_word_at)
-        ltac:(newest_memory_hyp) ltac:(lia || ZnWords.ZnWords).
-    let Hzero := match goal with H: _ <> 0 |- _ => H end in
-      rewrite <-word.unsigned_of_Z_0, !word.unsigned_inj_iff in Hzero by exact _;
-      rewrite !word.lor_0_iff, !word.broadcast_0_iff in Hzero.
+        ltac:(newest_memory_hyp) ltac:(lia || ZnWords).
+    let H := match goal with H: _ <> 0 |- _ => H end in rename H into Hzero.
+    rewrite <-(word.unsigned_of_Z_0 (width:=width)) in Hzero. rewrite word.unsigned_inj_iff in Hzero.
+    rewrite !word.lor_0_iff, !word.broadcast_0_iff in Hzero.
+
     destruct (iszero P) eqn:HP, (iszero Q) eqn:HQ in *; try intuition discriminate;
-      repeat match goal with
-             | H : _ = _ -> _ |- _ => specialize (H eq_refl)
-             | H : ?x = ?y -> _ |- _ => assert (x = y -> False) as _ by inversion 1; clear H
-             end;
-      subst x4; subst x5; subst x6;
-      rewrite ?Byte.map_xor_0_l in * by (ZnWords).
+    repeat match goal with
+      | H : ?x = ?y -> _ |- _ => assert (x = y -> False) as _ by
+          (destruct Bitwidth.width_cases as [W|W]; symmetry in W; destruct W; inversion 1); clear H
+      | H : ?x = ?y -> _ |- _ => assert (x = y) as Heqxy by (destruct Bitwidth.width_cases as [W|W]; symmetry in W; destruct W; exact eq_refl); specialize (H Heqxy); clear Heqxy
+    end; subst x4; subst x5; subst x6; rewrite ?Byte.map_xor_0_l in * by (ZnWords).
     { (* 0 + 0 *)
       eexists (exist _ (0,0,0)%F I); split.
-      { use_sep_assumption; cancel. reflexivity. }
+      { use_sep_assumption; cancel. destruct Bitwidth.width_cases as [W|W]; symmetry in W; destruct W; reflexivity. }
       apply Decidable.dec_bool, Jacobian.iszero_iff in HP.
       apply Decidable.dec_bool, Jacobian.iszero_iff in HQ.
       rewrite Jacobian.eq_iff, Jacobian.to_affine_add, HP, HQ.
@@ -415,13 +494,14 @@ Proof.
       eexists; split; [ecancel_assumption|].
       rewrite Jacobian.eq_iff, Jacobian.to_affine_add, Jacobian.to_affine_add_inequal_nz_nz; trivial; reflexivity. } }
   { (* if !ok *)
-    rewrite <-word.unsigned_of_Z_0, !word.unsigned_inj_iff in H27 by exact _.
+    rewrite <-(word.unsigned_of_Z_0 (width:=width)), !word.unsigned_inj_iff in H27 by exact _.
     rewrite !word.lor_0_iff, !word.broadcast_0_iff in H27.
     case H27 as ((HP&HQ)&->); rewrite ?HP, ?HQ in *;
       repeat match goal with
-             | H : _ = _ -> _ |- _ => specialize (H eq_refl)
-             | H : ?x = ?y -> _ |- _ => assert (x = y -> False) as _ by inversion 1; clear H
-             end;
+      | H : ?x = ?y -> _ |- _ => assert (x = y -> False) as _ by
+          (destruct Bitwidth.width_cases as [W|W]; symmetry in W; destruct W; inversion 1); clear H
+      | H : ?x = ?y -> _ |- _ => assert (x = y) as Heqxy by (destruct Bitwidth.width_cases as [W|W]; symmetry in W; destruct W; exact eq_refl); specialize (H Heqxy); clear Heqxy
+    end;
       subst x4; subst x5; subst x6;
       rewrite ?Byte.map_xor_0_l in * by (rewrite ?length_point; ZnWords.ZnWords).
     rewrite <-Bool.not_true_iff_false in HP, HQ.
@@ -435,9 +515,9 @@ Proof.
 
     straightline_call; repeat straightline; ssplit (* memcpy *).
     { ecancel_assumption. }
-    { rewrite H10, length_point; trivial. }
-    { trivial. }
-    { clear; ZnWords.ZnWords. }
+    { rewrite H10, length_point; ZnWords. }
+    { rewrite length_point. ZnWords. }
+    { ZnWords.ZnWords. }
     repeat straightline.
     (* stackdealloc *)
     progress repeat seprewrite_in_by (symmetry! @Array.array1_iff_eq_of_list_word_at)
@@ -468,68 +548,66 @@ Proof.
   cbv [id]. intros. assumption.
 Qed.
 
-Definition p256_point_double := func!(out, in1) {
-  stackalloc 32 as D;
-  stackalloc 32 as A;
-  stackalloc 32 as tmp;
-  p256_coord_add(D, in1.+$32, in1.+$32);
-  p256_coord_sqr(tmp, in1.+$32.+$32);
-  p256_coord_sqr(D, D);
-  p256_coord_mul(out.+$32.+$32, in1.+$32.+$32, in1.+$32);
-  p256_coord_add(out.+$32.+$32, out.+$32.+$32, out.+$32.+$32);
-  p256_coord_add(A, in1, tmp);
-  p256_coord_sub(tmp, in1, tmp);
-  { stackalloc 32 as t2; p256_coord_add(t2, tmp, tmp); p256_coord_add(tmp, t2, tmp) };
-  p256_coord_sqr(out.+$32, D);
-  p256_coord_mul(A, A, tmp);
-  p256_coord_mul(D, D, in1);
-  p256_coord_sqr(out, A);
-  p256_coord_add(tmp, D, D);
-  p256_coord_sub(out, out, tmp);
-  p256_coord_sub(D, D, out);
-  p256_coord_mul(D, D, A);
-  p256_coord_halve(out.+$32, out.+$32);
-  p256_coord_sub(out.+$32, D, out.+$32)
-}.
-
 Lemma p256_point_double_ok : program_logic_goal_for_function! p256_point_double.
 Proof.
   cbv [spec_of_p256_point_double].
   straightline; repeat straightline_cleanup.
   destruct P as (((x1 & y1) & z1) & p1);
     cbv [proj1_sig proj2_sig fst snd point.to_bytes] in * |-.
-  progress repeat seprewrite_in_by Array.sep_eq_of_list_word_at_app H18
-     ltac:(rewrite ?app_length, ?length_coord; trivial; try Lia.lia).
+  progress repeat seprewrite_in_by @Array.sep_eq_of_list_word_at_app H18
+     ltac:(rewrite ?app_length, ?length_coord; trivial; try ZnWords).
 
   repeat straightline.
-  repeat seprewrite_in_by Array.array1_iff_eq_of_list_word_at H18 ltac:(Lia.lia).
+
+  split.  { cbv delta [Memory.bytes_per_word]. destruct Bitwidth.width_cases as [W | W]; rewrite W; cbv; lia. }
+  repeat straightline.
+  split.  { cbv delta [Memory.bytes_per_word]. destruct Bitwidth.width_cases as [W | W]; rewrite W; cbv; lia. }
+  repeat straightline.
+  split.  { cbv delta [Memory.bytes_per_word]. destruct Bitwidth.width_cases as [W | W]; rewrite W; cbv; lia. }
+  repeat straightline.
+
+  repeat seprewrite_in_by @Array.array1_iff_eq_of_list_word_at H18 ltac:(ZnWords).
 
   rewrite <-(firstn_skipn 32 out) in H18.
   rewrite <-(firstn_skipn 32 (skipn _ out)) in H18.
   rewrite !skipn_skipn in H18.
 rewrite ?app_length, ?length_coord in *.
-  progress repeat seprewrite_in_by Array.sep_eq_of_list_word_at_app H18
-    ltac:(repeat rewrite ?app_length, ?firstn_length, ?skipn_length, ?Nat.min_l; try Lia.lia; trivial).
+  progress repeat seprewrite_in_by @Array.sep_eq_of_list_word_at_app H18
+    ltac:(repeat rewrite ?app_length, ?firstn_length, ?skipn_length, ?Nat.min_l; try ZnWords; trivial).
 
-  progress change (Z.of_nat 32) with 32 in *.
+  change (Z.of_nat 32) with 32 in *.
 
-  progress repeat (set (List.skipn  _ _) in H18 || set (List.firstn  _ _) in H18).
-
-  progress repeat (straightline_call; ssplit;
+  progress repeat (clear_old_memory_hyps; straightline_call; ssplit;
     [ solve [repeat match goal with
       | |- True => exact I
       | |- exists _, _ => letexists
-      | |- _ =>
-          repeat match goal with x := _ : list _ |- _ => subst x end;
-          progress rewrite ?length_coord, ?firstn_length, ?skipn_length; lia
+      | |- _ => progress rewrite ?length_coord, ?firstn_length, ?skipn_length; ZnWords
       | _ => ecancel_assumption
       end] ..
     | repeat straightline ]).
 
   (* stackalloc *)
-  repeat seprewrite_in_by Array.array1_iff_eq_of_list_word_at H42 ltac:(Lia.lia).
+  split.  { cbv delta [Memory.bytes_per_word]. destruct Bitwidth.width_cases as [W | W]; rewrite W; cbv; lia. }
+  repeat straightline.
+  repeat seprewrite_in_by @Array.array1_iff_eq_of_list_word_at ltac:(newest_memory_hyp) ltac:(ZnWords).
 
-  progress repeat (straightline_call; ssplit;
+  progress repeat (clear_old_memory_hyps; straightline_call; ssplit;
+    [ solve [repeat match goal with
+      | |- True => exact I
+      | |- exists _, _ => letexists
+      | |- _ => progress rewrite ?length_coord, ?firstn_length, ?skipn_length; ZnWords
+      | _ => ecancel_assumption
+      end] ..
+    | repeat straightline ]).
+
+  (* stackdealloc *)
+  progress repeat seprewrite_in_by (symmetry! @Array.array1_iff_eq_of_list_word_at) ltac:(newest_memory_hyp) ltac:(rewrite ?length_coord; ZnWords).
+  progress repeat match type of H32 with context [Array.array ptsto _ _ (coord.to_bytes ?x)] =>
+    unique pose proof (length_coord x) end.
+  repeat straightline.
+  progress repeat seprewrite_in_by (@Array.array1_iff_eq_of_list_word_at) ltac:(newest_memory_hyp) ltac:(rewrite ?length_coord; ZnWords).
+
+  progress repeat (clear_old_memory_hyps; straightline_call; ssplit;
     [ solve [repeat match goal with
       | |- True => exact I
       | |- exists _, _ => letexists
@@ -541,34 +619,17 @@ rewrite ?app_length, ?length_coord in *.
     | repeat straightline ]).
 
   (* stackdealloc *)
-  progress repeat seprewrite_in_by (symmetry! @Array.array1_iff_eq_of_list_word_at) H50 ltac:(rewrite ?length_coord; Lia.lia).
-  progress repeat match type of H50 with context [Array.array ptsto _ _ (coord.to_bytes ?x)] =>
+  progress repeat seprewrite_in_by (symmetry! @Array.array1_iff_eq_of_list_word_at) ltac:(newest_memory_hyp) ltac:(rewrite ?length_coord; ZnWords).
+  progress repeat match type of H41 with context [Array.array ptsto _ _ (coord.to_bytes ?x)] =>
     unique pose proof (length_coord x) end.
   repeat straightline.
-  progress repeat seprewrite_in_by (@Array.array1_iff_eq_of_list_word_at) H50 ltac:(rewrite ?length_coord; Lia.lia).
-
-  progress repeat (straightline_call; ssplit;
-    [ solve [repeat match goal with
-      | |- True => exact I
-      | |- exists _, _ => letexists
-      | |- _ =>
-          repeat match goal with x := _ : list _ |- _ => subst x end;
-          progress rewrite ?length_coord, ?firstn_length, ?skipn_length; lia
-      | _ => ecancel_assumption
-      end] ..
-    | repeat straightline ]).
-
-  (* stackdealloc *)
-  progress repeat seprewrite_in_by (symmetry! @Array.array1_iff_eq_of_list_word_at) H69 ltac:(rewrite ?length_coord; Lia.lia).
-  progress repeat match type of H69 with context [Array.array ptsto _ _ (coord.to_bytes ?x)] =>
-    unique pose proof (length_coord x) end.
-  repeat straightline.
-  progress repeat seprewrite_in_by (@Array.array1_iff_eq_of_list_word_at) H69 ltac:(rewrite ?length_coord; Lia.lia).
+  progress repeat seprewrite_in_by (@Array.array1_iff_eq_of_list_word_at) ltac:(newest_memory_hyp) ltac:(rewrite ?length_coord; ZnWords).
 
   (* postcondition *)
 
   cbv [proj1_sig proj2_sig fst snd point.to_bytes Jacobian.double_minus_3 Jacobian.double_minus3_impl Jacobian.Fsquare Jacobian.Ftriple Jacobian.Fhalve ].
-  progress repeat seprewrite_in_by Array.list_word_at_app_of_adjacent_eq H69 ltac:(rewrite ?length_coord; listZnWords).
-  rewrite ?F.pow_3_r, ?F.pow_2_r in H69.
+  progress repeat seprewrite_in_by @Array.list_word_at_app_of_adjacent_eq  ltac:(newest_memory_hyp) ltac:(rewrite ?length_coord; listZnWords).
+  rewrite ?F.pow_3_r, ?F.pow_2_r in H41.
   ecancel_assumption.
 Qed.
+End WithParameters.
