src/Bedrock/P256/Platform.v
@@ -1,4 +1,7 @@
 Require Import Bedrock.P256.Specs.
+Require Import Coq.ZArith.ZArith.
+From bedrock2 Require Import Loops.
+Require Import Bedrock.Field.Common.Tactics.
 
 Import Specs.NotationsCustomEntry Specs.coord Specs.point.
 
@@ -16,14 +19,15 @@ ProgramLogic WeakestPrecondition
 ProgramLogic.Coercions
 Word.Interface OfListWord Separation SeparationLogic
 letexists
-BasicC64Semantics
 ListIndexNotations
 SepAutoArray
 symmetry
 PeanoNat micromega.Lia
 Tactics
 UniquePose
-micromega.Lia Word.Properties.
+micromega.Lia Word.Properties
+ZnWords
+bedrock2.BasicCSemantics.
 
 Import ListIndexNotations.
 Local Open Scope list_index_scope.
@@ -33,7 +37,24 @@ Local Open Scope string_scope.
 Local Open Scope list_scope.
 
 Import (notations) coqutil.Map.Memory.
-Import bedrock2.wsize.
+Require Import bedrock2.wsize.
+
+
+Require coqutil.Word.Interface.
+Require coqutil.Map.Interface.
+
+(* Parameterize word size to ensure proofs are valid in 32 and 64 bit context.*)
+Section WithParameters.
+Context {width} {BW: Bitwidth.Bitwidth width}.
+#[local] Hint Extern 0 (word width) => exact (Naive.word width) : typeclass_instances.
+#[local] Notation word := (Naive.word width).
+
+Import Specs. (* Now word is accessible with short name. *)
+
+(* ZnWords with destructed word size equality after ZnWords_pre, to incorporate word size in hypothesis. *)
+#[local] Ltac ZnWords ::=
+  pose proof word_ok;
+  destruct Bitwidth.width_cases as [W|W]; symmetry in W; ZnWords_pre; try destruct W; better_lia.
 
 Definition br_value_barrier := func! (a) ~> a {
   /*skip*/ (* insert appropriate incantation for compilers that optimize values *)
@@ -73,7 +94,7 @@ Proof.
   cbv [word.broadcast]; apply f_equal.
   apply word.unsigned_inj, Z.bits_inj'; intros i Hi.
   rewrite word.unsigned_and, !word.unsigned_of_Z, !word.testbit_wrap.
-  f_equal. f_equal. change (word.wrap 1) with (Z.ones 1). rewrite Z.land_ones by lia.
+  f_equal. f_equal. replace (word.wrap 1) with (Z.ones 1) by (cbv [Z.ones]; ZnWords). rewrite Z.land_ones by lia.
   rewrite <-Z.bit0_mod, Z.bit0_odd; trivial.
 Qed.
 
@@ -83,7 +104,9 @@ Proof.
   repeat straightline.
   straightline_call; repeat straightline.
   subst y.
-  rewrite word.signed_lts, <-word.testbit_msb.
+  rewrite word.signed_lts.
+  rewrite word.signed_of_Z_nowrap by ZnWords.
+  rewrite <-word.testbit_msb.
   setoid_rewrite eval_wmask'.
   setoid_rewrite word.srs_msb; trivial.
 Qed.
@@ -93,14 +116,13 @@ Proof.
   cbv [spec_of_br_broadcast_nonzero].
   repeat straightline.
   straightline_call; repeat straightline.
-  apply f_equal, Bool.eq_true_iff_eq; rewrite Bool.negb_true_iff, Z.eqb_neq, <-word.nz_signed.
-  try rewrite word.sub_0_l.
-  rewrite word.signed_lts, word.signed_of_Z_nowrap by lia.
+  apply f_equal, Bool.eq_true_iff_eq; rewrite Bool.negb_true_iff, Z.eqb_neq.
+  rewrite word.signed_lts, word.signed_of_Z_nowrap by ZnWords.
   rewrite <-word.testbit_msb, word.unsigned_or_nowrap, Z.lor_spec, !word.testbit_msb.
+  rewrite <- nz_signed.
   case Z.ltb_spec; intros; cbn [orb]; try lia.
-  setoid_rewrite word.signed_opp_nowrap; intuition ZnWords.ZnWords.
+  setoid_rewrite signed_opp_nowrap; intuition ZnWords.ZnWords.
 Qed.
-
 
 Definition br_cmov := func! (c, vnz, vz) ~> r {
   unpack! m = br_broadcast_nonzero(c);
@@ -119,10 +141,13 @@ Proof.
     repeat rewrite ?word.unsigned_or, word.unsigned_and, ?word.unsigned_opp, ?word.unsigned_not, ?word.unsigned_of_Z_0, ?word.unsigned_of_Z_1; cbv [word.wrap].
   all : apply Z.bits_inj'; intros i Hi;
     repeat rewrite <-?Z.land_ones, ?Z.land_spec, ?Z.lor_spec, ?Z.testbit_ones, ?Z.lnot_spec, ?Z.testbit_0_l by try ZnWords.ZnWords.
+  2: rewrite word.unsigned_opp_nowrap, word.unsigned_of_Z_1 by ZnWords;
+     change (2 ^ width - 1) with (Z.pred (2 ^ width)); rewrite <- Z.ones_equiv.
   all: repeat (((case Z.ltb_spec; [|]; intros)||(case Z.leb_spec; [|]; intros)); rewrite
       ?Bool.andb_true_l, ?Bool.andb_true_r, ?Bool.orb_true_l, ?Bool.orb_true_r,
       ?Bool.andb_false_l, ?Bool.andb_false_r, ?Bool.orb_false_l, ?Bool.orb_false_r,
-      ?Z.testbit_0_l, ?prove_Zeq_bitwise.testbit_minus1, ?Z.testbit_neg_r, ?Z.testbit_high
+      ?Z.testbit_0_l, ?prove_Zeq_bitwise.testbit_minus1, ?Z.testbit_neg_r, ?Z.testbit_high,
+      ?Z.testbit_ones
     by intuition (idtac;
          match goal with
          | H : ?x < ?y^?a |- ?x < ?y^?b =>
@@ -138,14 +163,13 @@ Definition br_abs := func! (k, sign_mask) ~> r {
 }.
 
 #[local] Ltac div_mod_lia := rewrite ?word.signed_eq_swrap_unsigned, ?word.swrap_as_div_mod in *;
-      PreOmega.Z.to_euclidean_division_equations; lia.
+      PreOmega.Z.to_euclidean_division_equations; ZnWords.
 
 Lemma opp_sub_opp_add n m : - n - m = - (n + m). Proof. lia. Qed.
 
 Lemma br_abs_ok : program_logic_goal_for_function! br_abs.
 Proof.
   cbv [spec_of_br_abs]. repeat straightline.
-
   subst r.
   pose proof word.unsigned_range k.
   destruct (Z.abs_spec (word.signed k)) as [[? ->] | [? ->]].
@@ -158,12 +182,12 @@ Proof.
       ?word.unsigned_and_nowrap, ?word.unsigned_of_Z_nowrap,
       ?word.unsigned_xor_nowrap, ?Hsign, ?Z.land_ones; try (lia || ZnWords.ZnWords);
       try (case Z.ltb_spec; intros); try div_mod_lia.
-      all: rewrite Z.land_comm, Z.land_ones_low by (lia || cbv; trivial).
+      all: rewrite Z.land_comm, Z.land_ones_low; try ZnWords.
+      2, 4: clear -BW; destruct Bitwidth.width_cases as [-> | ->]; cbv; trivial.
       all: rewrite Z.lxor_comm, <- word.unsigned_not_nowrap, word.unsigned_not;
-        rewrite Zbitwise.Z.lnot_eq_pred_opp; cbn.
-      all: unfold word.wrap;
-        rewrite opp_sub_opp_add, Modulo.Z.mod_opp_small by ZnWords.ZnWords.
-      all: div_mod_lia. }
+        rewrite Zbitwise.Z.lnot_eq_pred_opp.
+      all: cbv [word.wrap]; rewrite opp_sub_opp_add, Modulo.Z.mod_opp_small by ZnWords.
+      all: try div_mod_lia. }
 Qed.
 
 Definition br_memset := func! (p_d, v, n) {
@@ -187,4 +211,8 @@ Lemma br_memset_ok : program_logic_goal_for_function! br_memset.
 Admitted.
 
 Lemma br_memcxor_ok : program_logic_goal_for_function! br_memcxor.
+Proof.
+  (* Proof implementation for br_memcxor would go here *)
 Admitted.
+
+End WithParameters.
